\input{../cs164.tex}
\usepackage{amsmath, verbatim, tikz, float, dsfont}

\oddsidemargin 0in
\evensidemargin 0in
\textwidth 6.5in
\topmargin -0.5in
\textheight 9.0in
\newcommand{\norm}[1]{\left\lVert #1 \right\rVert}
\newcommand{\?}{\stackrel{?}{=}}

\begin{document}

\solution{Nikhil Unni (cs164-es), Section : Monday 3pm}{WA3}{Fall 2015}
\pagestyle{myheadings}


\begin{enumerate}
    \item 
          \begin{enumerate}
          \item
                $$A \rightarrow B C A' | C A'$$
                $$A' \rightarrow B C A' | \epsilon$$
                $$B \rightarrow int | (A)$$
                $$C \rightarrow bool$$

          \item
                $$L \rightarrow bool M$$
                $$M \rightarrow + N | \epsilon$$
                $$N \rightarrow bool | int$$

          \item
                $$A \rightarrow int B$$
                $$B \rightarrow + A$$
                $$B \rightarrow - C$$
                $$B \rightarrow \epsilon$$
                $$C \rightarrow A$$
                $$C \rightarrow (A)$$
          \end{enumerate}

    \item Consider the following grammar describing a certain sort of parenthesis:
          $$A \rightarrow \epsilon | A + B | C + C$$
          $$B \rightarrow C | C * B$$
          $$C \rightarrow (A) | int$$

          \begin{enumerate}
          \item Left-factor this grammar.\\
                $$A \rightarrow C + CA' | A'$$
                $$A' \rightarrow + B A' | \epsilon$$
                $$B \rightarrow C B'$$
                $$Follow \rightarrow * B | \epsilon$$
                $$C \rightarrow (A) | int$$

          \item Give the First and Follow sets for each nonterminal for the grammar in part (a).\\

          First(A) = $\{(,$ int, $+\}$\\
          First($A'$) = $\{+\}$\\
          First(B) = $\{(,$ int$\}$\\
          First($B'$) = $\{*\}$\\
          First(C) = $\{(,$ int$\}$\\

          Follow(A) = $\{), \$\}$\\
          Follow($A'$) = $\{), \$\}$\\
          Follow(B) = $\{), +, \$\}$\\
          Follow($B'$) = $\{),+, \$\}$\\
          Follow(C) = $\{), +, *, \$\}$\\


          \item Is there a conflict in the original grammar?\\\\

          Yes -- besides the left recursion, there’s a first/first conflict between first(A) and first(C), which are both transitions from A. Also, there’s another first/first conflict on B between the two C transitions.

          \item Using the information, construct an LL parsing table for the grammar obtained in (a).

          \begin{center}
            \begin{tabular}{ c|c|c|c|c|c|c } 
                 & $+$ & $*$ & $($ & $)$ & int & $\$$\\
               \hline
               A & $A'$ & & $C + CA'$ & $A'$ & $C + CA'$ & $A'$\\
               $A'$ & $+BA'$ & & & $\epsilon$ & & $\epsilon$\\
               B & & & $CB'$ & & $CB'$\\
               $B'$ & $\epsilon$ & $*B$ & & $\epsilon$ & & $\epsilon$\\
               C & & & (A) & & int\\
               \hline
            \end{tabular}
          \end{center}

          \item What would go wrong if we tried to parse the following input string?
          $$((int + int) + int)+int+)$$\\\\

          We'll continue to parse until our stack is $A'\$$, and our remaining input is ``+)''. Going forward this becomes :
          $$+BA'\$ , +)$$
          $$BA'\$ , ) $$

          At this point, there is no table entry for T[B,$)$], so we get an error on the input.
          \end{enumerate}

      \item Complete the table below showing the trace of an LR(1) parser on the input provided.
          \begin{center}
            \begin{tabular}{c c c}
               Stack & Input & Action\\
               \hline
                 & $\triangleright$ x + x + + x + $\$$ & shift\\
                 x & x $\triangleright$ + x + + x + $\$$ & reduce ($B \rightarrow x$)\\
                 B & x $\triangleright$ + x + + x + $\$$& shift 2\\
                 B + x & x + x $\triangleright$ + + x + $\$$ & reduce ($B \rightarrow x$)\\
                 B + B & x + x $\triangleright$ + + x + $\$$ & shift 3\\
                 B + B + + x & x + x + + x $\triangleright$ + $\$$ & reduce ($B \rightarrow x$)\\
                 B + B + + B & x + x + + x $\triangleright$ + $\$$ & shift 1\\
                 B + B + + B + & x + x + + x + $\triangleright$ $\$$ & reduce ($A \rightarrow +B+$)\\
                 B + B + A & x + x + + x + $\triangleright$ $\$$ & reduce ($A \rightarrow B + A$)\\
                 B + A & x + x + + x + $\triangleright$ $\$$ & reduce ($A \rightarrow B + A$)\\
                 A & x + x + + x + $\triangleright$ $\$$ & reduce ($S \rightarrow A$)\\
                 S & x + x + + x + $\triangleright$ $\$$ & accept\\
               
            \end{tabular}
          \end{center}

\end{enumerate}

\end{document}
